## Theorem: algebraic properties of sets

**Commutative**:

* $S_{1} \cup S_{2} = S_{2} \cup S_{1}$
* $S_{1} \cap S_{2} = S_{2} \cap S_{1}$

**Associative**:

* $S_{1} \cup (S_{2} \cup S_{3}) = (S_{1} \cup S_{2}) \cup S_{3}$
* $S_{1} \cap (S_{2} \cap S_{3}) = (S_{1} \cap S_{2}) \cap S_{3}$

**Distributive**:

* $S_{1} \cup (S_{2} \cap S_{3}) = (S_{1} \cap S_{2}) \cup (S_{1} \cap S_{3})$
* $S_{1} \cap (S_{2} \cup S_{3}) = (S_{1} \cup S_{2}) \cap (S_{1} \cup S_{3})$

**Idempotent**:

* $S_{1} \cup S_{1} = S_{1}$
* $S_{1} \cap S_{1} = S_{1}$

**Complement rules**:

* $\overline{(\overline{S_{1}})} = S_{1}$
* $S_{1} \cup \overline{S_{1}} = U$
* $S_{1} \cap \overline{S_{1}} = \emptyset$
* $\overline{\emptyset} = U$
* $\overline{U} = \emptyset$
* $\overline{S_{1} \cup S_{2}} = \overline{S_{1}} \cap \overline{S_{2}}$
* $\overline{S_{1} \cap S_{2}} = \overline{S_{1}} \cup \overline{S_{2}}$

**Universal rules**:

* $S_{1} \cup U = U$
* $S_{1} \cap U = S_{1}$

**Null rules**:

* $S_{1} \cup \emptyset = S_{1}$
* $S_{1} \cap \emptyset = \emptyset$

**End theorem.**

---

## Proof